Continue work on shifts

language_formalisation/substitution/substitution.v
@@ -7,38 +7,38 @@ Module Sub.
 
 Fixpoint v_shift (v : val) d (cut : nat) :=
 match v with
-| Var (x, n) => if cut <=? n then Var (x, n + d) else Var (x, n)
+| Var (x, n) => if cut <=? n then Var (x, d + n) else Var (x, n)
 | Unit => Unit
 | Int n => Int n
 | Inl v' => Inl (v_shift v' d cut)
 | Inr v' => Inr (v_shift v' d cut)
 | Pair v1 v2 => Pair (v_shift v1 d cut) (v_shift v2 d cut)
-| Fun x c => Fun x (c_shift c d (cut+1))
-| Handler x c_ret h => Handler x (c_shift c_ret d (cut+1)) (h_shift h d cut)
+| Fun x c => Fun x (c_shift c d (1+cut))
+| Handler x c_ret h => Handler x (c_shift c_ret d (1+cut)) (h_shift h d cut)
 end
 with c_shift (c : comp) d (cut : nat) :=
 match c with
 | Ret v => Ret (v_shift v d cut)
 | Absurd v => Absurd (v_shift v d cut)
-| ΠMatch v x y c => ΠMatch (v_shift v d cut) x y (c_shift c d (cut+2))
+| ΠMatch v x y c => ΠMatch (v_shift v d cut) x y (c_shift c d (2+cut))
 | ΣMatch v xl cl xr cr =>
     ΣMatch (v_shift v d cut)
-      xl (c_shift cl d (cut+1))
-      xr (c_shift cr d (cut+1))
+      xl (c_shift cl d (1+cut))
+      xr (c_shift cr d (1+cut))
 | App v1 v2 => App (v_shift v1 d cut) (v_shift v2 d cut)
-| Op op v_arg y c => Op op (v_shift v_arg d cut) y (c_shift c d (cut+1))
-| LetRec f x c1 c2 => LetRec f x (c_shift c1 d (cut+2)) (c_shift c2 d (cut+1))
-| DoBind x c1 c2 => DoBind x (c_shift c1 d cut) (c_shift c2 d (cut+1))
+| Op op v_arg y c => Op op (v_shift v_arg d cut) y (c_shift c d (1+cut))
+| LetRec f x c1 c2 => LetRec f x (c_shift c1 d (2+cut)) (c_shift c2 d (1+cut))
+| DoBind x c1 c2 => DoBind x (c_shift c1 d cut) (c_shift c2 d (1+cut))
 | Handle v c' => Handle (v_shift v d cut) (c_shift c' d cut)
 end
 with h_shift (h : hcases) d (cut : nat) :=
 match h with
 | CasesØ => CasesØ
-| CasesU h op x k c => CasesU (h_shift h d cut) op x k (c_shift c d (cut+2))
+| CasesU h op x k c => CasesU (h_shift h d cut) op x k (c_shift c d (2+cut))
 end.
 
 Fixpoint sub_shift (sub : nat * val) d :=
-  let (db_i, v_s) := sub in (db_i + d, v_shift v_s d 0).
+  let (db_i, v_s) := sub in (d + db_i, v_shift v_s d 0).
 
 Fixpoint v_negshift (v : val) d (cut : nat) :=
 match v with
@@ -49,31 +49,31 @@ match v with
 | Inl v' => Inl (v_negshift v' d cut)
 | Inr v' => Inr (v_negshift v' d cut)
 | Pair v1 v2 => Pair (v_negshift v1 d cut) (v_negshift v2 d cut)
-| Fun x c => Fun x (c_negshift c d (cut+1))
+| Fun x c => Fun x (c_negshift c d (1+cut))
 | Handler x c_ret h =>
-    Handler x (c_negshift c_ret d (cut+1)) (h_negshift h d cut)
+    Handler x (c_negshift c_ret d (1+cut)) (h_negshift h d cut)
 end
 with c_negshift (c : comp) d (cut : nat) :=
 match c with
 | Ret v => Ret (v_negshift v d cut)
 | Absurd v => Absurd (v_negshift v d cut)
-| ΠMatch v x y c => ΠMatch (v_negshift v d cut) x y (c_negshift c d (cut+2))
+| ΠMatch v x y c => ΠMatch (v_negshift v d cut) x y (c_negshift c d (2+cut))
 | ΣMatch v xl cl xr cr =>
     ΣMatch (v_negshift v d cut)
-      xl (c_negshift cl d (cut+1))
-      xr (c_negshift cr d (cut+1))
+      xl (c_negshift cl d (1+cut))
+      xr (c_negshift cr d (1+cut))
 | App v1 v2 => App (v_negshift v1 d cut) (v_negshift v2 d cut)
-| Op op v_arg y c => Op op (v_negshift v_arg d cut) y (c_negshift c d (cut+1))
+| Op op v_arg y c => Op op (v_negshift v_arg d cut) y (c_negshift c d (1+cut))
 | LetRec f x c1 c2 =>
-    LetRec f x (c_negshift c1 d (cut+2)) (c_negshift c2 d (cut+1))
-| DoBind x c1 c2 => DoBind x (c_negshift c1 d cut) (c_negshift c2 d (cut+1))
+    LetRec f x (c_negshift c1 d (2+cut)) (c_negshift c2 d (1+cut))
+| DoBind x c1 c2 => DoBind x (c_negshift c1 d cut) (c_negshift c2 d (1+cut))
 | Handle v c' => Handle (v_negshift v d cut) (c_negshift c' d cut)
 end
 with h_negshift (h : hcases) d (cut : nat) :=
 match h with
 | CasesØ => CasesØ
 | CasesU h op x k c => 
-    CasesU (h_negshift h d cut) op x k (c_negshift c d (cut+2))
+    CasesU (h_negshift h d cut) op x k (c_negshift c d (2+cut))
 end.
 
 Fixpoint v_sub (v : val) (sub : nat * val) :=
