language_formalisation/substitution/substitution_lemmas.v
@@ -22,7 +22,7 @@ revert cut. induction v; intros cut; simpl; f_equal.
   destruct v as (name, db_i).
   destruct (cut <=? db_i) eqn:cmp; simpl.
   - apply (leb_complete _ _) in cmp.
-    assert (cut <= db_i + n) by omega.
+    assert (cut <= n + db_i) by omega.
     apply leb_correct in H. rewrite H.
     f_equal. f_equal. omega.
   - rewrite cmp. reflexivity. }
@@ -39,6 +39,46 @@ reflexivity. apply IHh. apply c_shift_shift.
 }
 Qed.
 
+Lemma v_shift_shift_alt n m cut (v:val) :
+  Sub.v_shift (Sub.v_shift v n cut) m (n+cut) = (Sub.v_shift v (n + m) cut)
+
+with c_shift_shift_alt n m cut (c:comp) :
+  Sub.c_shift (Sub.c_shift c n cut) m (n+cut) = (Sub.c_shift c (n + m) cut)
+
+with h_shift_shift_alt n m cut (h:hcases) :
+  Sub.h_shift (Sub.h_shift h n cut) m (n+cut) = (Sub.h_shift h (n + m) cut).
+Proof.
+{
+clear v_shift_shift_alt.
+revert cut. induction v; intros cut; simpl; f_equal.
+{ (* The only relevant case. *)
+  destruct v as (name, db_i).
+  destruct (cut <=? db_i) eqn:cmp; simpl.
+  - apply (leb_complete _ _) in cmp.
+    assert (n+cut <= n+db_i) by omega.
+    apply leb_correct in H. rewrite H.
+    f_equal. f_equal. omega.
+  - assert (n+cut <=? db_i = false).
+    { apply leb_correct_conv. apply leb_complete_conv in cmp. omega. }
+    rewrite H. reflexivity. }
+all : try reflexivity || apply IHv || apply IHv1 || apply IHv2.
+all : assert (S(n+cut)=n + S cut) by omega; try rewrite H.
+all : try apply c_shift_shift_alt || apply h_shift_shift_alt; assumption.
+}{
+clear c_shift_shift_alt.
+revert cut. induction c; intros cut; try destruct p; simpl; f_equal;
+try apply v_shift_shift_alt.
+all : assert (S(n+cut)=n + S cut) by omega; try rewrite H.
+all : assert (S(n+ S cut)=n + S (S cut)) by omega; try rewrite H0.
+all : try apply IHc || apply IHc1 || apply IHc2.
+}{
+clear h_shift_shift_alt.
+revert cut. induction h; intros cut; simpl; f_equal.
+reflexivity. apply IHh.
+assert (S(S(n+cut))=n+S(S cut)) by omega. rewrite H. 
+apply c_shift_shift_alt.
+}
+Qed.
 
 Lemma v_shift_makes_no_var v j:
   v_no_var_j (Sub.v_shift v 1 j) j
@@ -62,13 +102,13 @@ revert j; induction h; intros j; simpl; auto.
 Qed.
 
 Lemma v_no_var_shift (v:val) j cut:
-  v_no_var_j v j -> (cut <= j) -> v_no_var_j (Sub.v_shift v 1 cut) (j+1)
+  v_no_var_j v j -> (cut <= j) -> v_no_var_j (Sub.v_shift v 1 cut) (1+j)
 
 with c_no_var_shift (c:comp) j cut:
-  c_no_var_j c j -> (cut <= j) -> c_no_var_j (Sub.c_shift c 1 cut) (j+1)
+  c_no_var_j c j -> (cut <= j) -> c_no_var_j (Sub.c_shift c 1 cut) (1+j)
   
 with h_no_var_shift (h:hcases) j cut:
-  h_no_var_j h j -> (cut <= j) -> h_no_var_j (Sub.h_shift h 1 cut) (j+1).
+  h_no_var_j h j -> (cut <= j) -> h_no_var_j (Sub.h_shift h 1 cut) (1+j).
 Proof.
 {
 clear v_no_var_shift.
@@ -83,15 +123,11 @@ clear c_no_var_shift.
 revert j cut. induction c; intros j cut orig_clean j_le_cut; simpl; simpl in *; 
 try destruct p; try inv orig_clean; try constructor; try constructor; auto;
 try apply IHc || apply IHc1 || apply IHc2; try omega; auto.
-+ assert (j+1+2=j+2+1) by omega. rewrite H1. apply IHc. assumption. omega.
-+ inv H0. assumption.
-+ inv H0. assumption.
-+ assert (j+1+2=j+2+1) by omega. rewrite H1. apply IHc1. assumption. omega.
+all: inv H0; assumption.
 }{
 clear h_no_var_shift.
 revert j cut. induction h; intros j cut orig_clean j_le_cut; simpl;
 destruct orig_clean; auto. constructor. auto.
-assert (j+1+2=j+2+1) by omega. rewrite H1.
 apply c_no_var_shift. assumption. omega.
 }
 Qed.
@@ -108,8 +144,8 @@ with h_no_var_sub (h:hcases) j v_s :
 Proof.
 {
 clear v_no_var_sub.
-revert j. induction v; intros j v_s_clean; simpl; try constructor;
-try (apply IHv; assumption); auto.
+revert j. induction v; intros j v_s_clean; try constructor.
+all: try (apply IHv; assumption); auto.
 - destruct v as (x, n). simpl.
   induction (n =? j) eqn:fits.
   + assumption.
@@ -123,20 +159,18 @@ try destruct p; simpl; try constructor; auto;
 try apply IHc || apply IHc1 || apply IHc2;
 try (apply v_no_var_shift; assumption || omega).
 all:
-assert (v_no_var_j (Sub.v_shift v_s 1 0) (j + 1)) by
+assert (v_no_var_j (Sub.v_shift v_s 1 0) (1 + j)) by
   (apply v_no_var_shift; auto || omega);
-apply (v_no_var_shift _ _ 0) in H; try omega;
-simpl in H; rewrite v_shift_shift in H; simpl in H;
-assert (j+1+1=j+2) by omega; rewrite H0 in H; assumption.
+apply (v_no_var_shift _ _ 0) in H; try omega.
+all: rewrite v_shift_shift in H; simpl in H; assumption.
 }{
 clear h_no_var_sub.
 revert j v_s. induction h; intros j v_s v_s_clean; simpl; auto.
 constructor. auto.
-assert (v_no_var_j (Sub.v_shift v_s 1 0) (j + 1)).
+assert (v_no_var_j (Sub.v_shift v_s 1 0) (1+j)).
 { apply v_no_var_shift. auto. omega. }
-apply (v_no_var_shift _ _ 0) in H. simpl in H.
-rewrite (v_shift_shift _ _ _) in H.
-assert (j+1+1=j+2) by omega. rewrite H0 in H. auto. omega.
+apply (v_no_var_shift _ _ 0) in H.
+rewrite (v_shift_shift _ _ _) in H. auto. omega.
 }
 Qed.
 
@@ -150,7 +184,7 @@ Qed.
 Lemma h_shift_find_op_Some h o i j x k cop :
   find_op_case h o = Some (x, k, cop) -> 
   find_op_case (Sub.h_shift h i j) o = 
-    Some (x, k, (Sub.c_shift cop i (j+2))).
+    Some (x, k, (Sub.c_shift cop i (2+j))).
 Proof.
 intro; induction h.
 + simpl in H. discriminate.
@@ -162,15 +196,15 @@ Qed.
 (* needed for tmpl handling *)
 Lemma v_shift_comm_aux n i j d (v:val) :
 i >= j ->
-Sub.v_shift (Sub.v_shift v n i) d j = Sub.v_shift (Sub.v_shift v d j) n (i+d)
+Sub.v_shift (Sub.v_shift v n i) d j = Sub.v_shift (Sub.v_shift v d j) n (d+i)
 
 with c_shift_comm_aux n i j d (c:comp) :
 i >= j ->
-Sub.c_shift (Sub.c_shift c n i) d j = Sub.c_shift (Sub.c_shift c d j) n (i+d)
+Sub.c_shift (Sub.c_shift c n i) d j = Sub.c_shift (Sub.c_shift c d j) n (d+i)
 
 with h_shift_comm_aux n i j d (h:hcases) :
 i >= j ->
-Sub.h_shift (Sub.h_shift h n i) d j = Sub.h_shift (Sub.h_shift h d j) n (i+d).
+Sub.h_shift (Sub.h_shift h n i) d j = Sub.h_shift (Sub.h_shift h d j) n (d+i).
 Proof.
 {
 intros cmp. induction v; simpl.
@@ -178,35 +212,36 @@ intros cmp. induction v; simpl.
   clear v_shift_comm_aux c_shift_comm_aux h_shift_comm_aux.
   destruct v as (x, dbi).
   destruct (i<=?dbi) eqn:cmpi; destruct (j<=?dbi) eqn:cmpj; simpl;
-  destruct (i+d<=?dbi) eqn:cmpid; destruct (j<=?dbi+n) eqn:cmpjn; simpl;
-  destruct (i+d<=?dbi+d) eqn:cmpidd; simpl;
+  destruct (d+i<=?dbi) eqn:cmpid; destruct (j<=?n+dbi) eqn:cmpjn; simpl;
+  destruct (d+i<=?d+dbi) eqn:cmpidd; simpl;
   apply leb_complete in cmpj || apply leb_complete_conv in cmpj;
   apply leb_complete in cmpi || apply leb_complete_conv in cmpi;
   apply leb_complete in cmpjn || apply leb_complete_conv in cmpjn;
   apply leb_complete in cmpid || apply leb_complete_conv in cmpid;
   apply leb_complete in cmpidd || apply leb_complete_conv in cmpidd;
   try omega; simpl.  f_equal. f_equal. omega. f_equal. f_equal. omega.
-  + assert (j<=?dbi=true) by (apply leb_correct in cmpj; assumption).
-    rewrite H. auto.
-  + assert (j<=?dbi=false) by (apply leb_correct_conv in cmpj; assumption).
-    rewrite H. auto.
-  + assert (j<=?dbi=false) by (apply leb_correct_conv in cmpj; assumption).
-    rewrite H. auto. 
+  { assert (j<=?dbi=true) by (apply leb_correct in cmpj; assumption).
+    rewrite H. auto. }
+  all: assert (j<=?dbi=false) by (apply leb_correct_conv in cmpj; assumption).
+  all: rewrite H; auto.
 }
+clear v_shift_comm_aux h_shift_comm_aux.
 all: f_equal; auto.
-+ assert (i+d+1=i+1+d) by omega. rewrite H. eapply c_shift_comm_aux. omega.
-+ assert (i+d+1=i+1+d) by omega. rewrite H. eapply c_shift_comm_aux. omega.
+all: assert (S(d+i)=d+S i) by omega; rewrite H. 
+all: eapply c_shift_comm_aux; omega.
 }{
 intros cmp. induction c; simpl; f_equal; auto; 
-try eapply c_shift_comm_aux; try omega;
-assert (i+d+1=i+1+d) by omega; try rewrite H;
-assert (2=1+1) by omega; assert (i+d+(1+1)=i+(1+1)+d) by omega;
-try rewrite H0; try rewrite H1; eapply c_shift_comm_aux; omega.
+clear v_shift_comm_aux h_shift_comm_aux.
+try eapply c_shift_comm_aux; try omega.
+all: assert (S(d+i)=d+S i) by omega; try rewrite H.
+all: assert (S(d+S i)=d+S(S i)) by omega; try rewrite H0.
+all: eapply c_shift_comm_aux; omega.
 }{
+clear v_shift_comm_aux h_shift_comm_aux.
 intros cmp. induction h; simpl.
 all: f_equal; auto.
-assert (2=1+1) by omega; assert (i+d+(1+1)=i+(1+1)+d) by omega;
-rewrite H; rewrite H0; eapply c_shift_comm_aux; omega.
+assert (S(S(d+i))=d+S(S i)) by omega;
+rewrite H; eapply c_shift_comm_aux; omega.
 }
 Qed.
 
@@ -230,9 +265,8 @@ revert cut. induction v; intros cut m_le_n; simpl; f_equal.
   destruct v as (name, db_i). simpl.
   induction (cut <=? db_i) eqn:cmp; simpl.
   - apply (leb_complete _ _) in cmp.
-    assert (cut <= db_i + 1) by omega.
-    assert (cut <= db_i + n) by omega.
-    apply (leb_correct _ _) in H0. rewrite H0.
+    assert (cut <= n + db_i) by omega.
+    apply (leb_correct _ _) in H. rewrite H.
     f_equal. f_equal. omega.
   - rewrite cmp. reflexivity. }
 all : try reflexivity || apply IHv || apply IHv1 || apply IHv2.
@@ -259,8 +293,6 @@ clear v_shift_0.
 revert cut. induction v; intros cut;
 simpl; try (specialize (IHv cut)); try rewrite IHv; try reflexivity.
 + destruct v. simpl. destruct (cut <=? v0); try reflexivity.
-  assert (v0 + 0 = v0) by omega.
-  rewrite H; reflexivity.
 + rewrite IHv1, IHv2. reflexivity.
 + rewrite c_shift_0. reflexivity.
 + f_equal; try apply c_shift_0 || apply h_shift_0.
@@ -277,15 +309,15 @@ reflexivity. apply IHh. apply c_shift_0.
 Qed.
 
 
-Lemma v_shift_sub v v' i j (safe: j < i): 
+Lemma v_shift_sub v v' i j (safe: j <= i): 
   Sub.v_shift (v_sub v v' j) 1 i = 
-  (v_sub (Sub.v_shift v 1 (i+1)) (Sub.v_shift v' 1 i) j)
-with c_shift_sub c v' i j (safe: j < i): 
+  (v_sub (Sub.v_shift v 1 (1+i)) (Sub.v_shift v' 1 i) j)
+with c_shift_sub c v' i j (safe: j <= i): 
   Sub.c_shift (c_sub c v' j) 1 i = 
-  (c_sub (Sub.c_shift c 1 (i+1)) (Sub.v_shift v' 1 i) j)
-with h_shift_sub h v' i j (safe: j < i): 
+  (c_sub (Sub.c_shift c 1 (1+i)) (Sub.v_shift v' 1 i) j)
+with h_shift_sub h v' i j (safe: j <= i): 
   Sub.h_shift (h_sub h v' j) 1 i = 
-  (h_sub (Sub.h_shift h 1 (i+1)) (Sub.v_shift v' 1 i) j).
+  (h_sub (Sub.h_shift h 1 (1+i)) (Sub.v_shift v' 1 i) j).
 Proof.
 {
 induction v; unfold v_sub; simpl.
@@ -294,39 +326,54 @@ clear v_shift_sub c_shift_sub h_shift_sub.
 destruct v as (x, n). 
 destruct (n=?i) eqn:ni.
 apply Nat.eqb_eq in ni. subst.
-++ assert (i=?j=false) by (apply Nat.eqb_neq; omega).
-  rewrite H. assert (i+1<=?i=false) by (apply leb_correct_conv; omega).
-  rewrite H0. simpl. assert (j<=?i=true) by (apply leb_correct;omega).
-  rewrite H1. assert (i=?j=false) by (apply Nat.eqb_neq; omega).
-  rewrite H2. simpl. rewrite H1. assert (i<=?i-1=false).
-  apply leb_correct_conv. omega. rewrite H3. reflexivity.
+++
+  destruct (i=?j) eqn:eqij.
+  {
+    apply Nat.eqb_eq in eqij. subst.
+    assert (1+j<=?j=false) by (apply leb_correct_conv; omega).
+    simpl in H. rewrite H. simpl.
+    assert (j=?j=true) by (apply Nat.eqb_eq; reflexivity).
+    rewrite H0. simpl. 
+    rewrite v_negshift_shift. rewrite v_negshift_shift.
+    rewrite v_shift_shift. rewrite v_shift_shift. f_equal.
+    omega. omega.
+  }
+  assert (1+i<=?i=false) by (apply leb_correct_conv; omega).
+  simpl in H. rewrite H. simpl.
+  assert (j<=?i=true) by (apply leb_correct;omega).
+  rewrite H0. rewrite eqij. simpl. rewrite H0.
+  assert (i<=?i-1=false).
+  { apply leb_correct_conv. apply Nat.eqb_neq in eqij. 
+    apply leb_complete in H0. omega. }
+  rewrite H1. reflexivity.
 ++ destruct (n=?j) eqn:nj.
 + apply Nat.eqb_eq in nj. subst.
-  assert (i+1<=?j=false) by (apply leb_correct_conv; omega).
-  rewrite H. simpl. assert (j=?j=true) by (apply Nat.eqb_eq; omega).
-  rewrite H0. rewrite v_negshift_shift. rewrite v_negshift_shift.
-  assert (1-1=0) by omega. rewrite H1. rewrite v_shift_0. rewrite v_shift_0.
+  assert (1+i<=?j=false) by (apply leb_correct_conv; omega).
+  simpl in H. rewrite H.
+  simpl. assert (j=?j=true) by (apply Nat.eqb_eq; omega).
+  rewrite H0. rewrite v_negshift_shift. rewrite v_negshift_shift. simpl.
+  rewrite v_shift_0. rewrite v_shift_0.
   reflexivity. omega. omega.
 + destruct (i<=?n) eqn:iln; simpl.
   - destruct (j<=?n) eqn:jln; simpl.
     * apply leb_complete in jln. apply leb_complete in iln.
       assert (i<=?n-1=true).
       { apply leb_correct. apply Nat.eqb_neq in ni. omega. }
-      rewrite H. simpl. assert (i+1<=?n=true).
-      { apply leb_correct. apply leb_complete in H. omega. }
-      rewrite H0. simpl. 
-      assert (n+1=?j=false).
+      rewrite H. simpl. assert (1+i<=?n=true).
+      { apply leb_correct. apply leb_complete in H.
+        apply Nat.eqb_neq in ni. omega. }
+      simpl in H0. rewrite H0. simpl. 
+      assert (1+n=?j=false).
       { apply Nat.eqb_neq. omega. }
-      rewrite H1. simpl. assert (j<=?n+1=true).
+      simpl in H1. rewrite H1. simpl. assert (j<=? S n=true).
       { apply leb_correct. omega. }
       rewrite H2. simpl.
-      f_equal. f_equal. assert (n>0) by omega. omega.
-    * rewrite iln. apply leb_complete in iln. assert (i+1<=?n=true).
-      { apply leb_correct. apply Nat.eqb_neq in ni. omega. }
-      rewrite H. apply leb_complete in H. apply leb_complete_conv in jln. omega. 
+      f_equal. f_equal. assert (n>0) by (apply Nat.eqb_neq in ni; omega).
+      omega.
+    * apply leb_complete in iln. apply leb_complete_conv in jln. omega.
   - apply leb_complete_conv in iln.
-    assert (i+1<=?n=false) by (apply leb_correct_conv; omega).
-    rewrite H. simpl. rewrite nj. simpl.
+    assert (1+i<=?n=false) by (apply leb_correct_conv; omega).
+    simpl in H. rewrite H. simpl. rewrite nj. simpl.
     destruct (j<=?n) eqn:jln.
     * simpl. assert (i<=?n-1=false).
       { apply leb_correct_conv. omega. }
@@ -349,12 +396,12 @@ induction c; unfold c_sub; simpl; f_equal;
 try apply v_shift_sub; try assumption.
 + clear v_shift_sub h_shift_sub.
   unfold c_sub in c_shift_sub. rewrite <-(v_shift_shift 1).
-  rewrite (v_shift_comm_aux 1 j). rewrite (v_shift_comm_aux 1 (j+1)).
-  assert (j+1+1=j+2) by omega. rewrite H. rewrite c_shift_sub. clear c_shift_sub.
-  f_equal. f_equal. f_equal. all: try omega.
+  rewrite (v_shift_comm_aux 1 j). rewrite (v_shift_comm_aux 1 (1+j)). simpl.
+  rewrite c_shift_sub. clear c_shift_sub.
+  f_equal. f_equal. all: try omega.
   rewrite <-(v_shift_shift 1 1 0). rewrite (v_shift_comm_aux 1 j).
-  rewrite (v_shift_comm_aux 1 (j+1)). f_equal. rewrite (v_shift_comm_aux 1 i).
-  rewrite (v_shift_comm_aux 1 (i+1)). f_equal. f_equal. all: omega.
+  rewrite (v_shift_comm_aux 1 (1+j)). f_equal. rewrite (v_shift_comm_aux 1 i).
+  rewrite (v_shift_comm_aux 1 (1+i)). f_equal. f_equal. all: omega.
 + clear v_shift_sub h_shift_sub.
   unfold c_sub in c_shift_sub. rewrite v_shift_comm_aux. rewrite c_shift_sub.
   f_equal. f_equal. f_equal. rewrite (v_shift_comm_aux 1 j). f_equal.
@@ -369,12 +416,12 @@ try apply v_shift_sub; try assumption.
   rewrite (v_shift_comm_aux 1 i). f_equal. all: omega.
 + clear v_shift_sub h_shift_sub.
   unfold c_sub in c_shift_sub. rewrite <-(v_shift_shift 1).
-  rewrite (v_shift_comm_aux 1 j). rewrite (v_shift_comm_aux 1 (j+1)).
-  assert (j+1+1=j+2) by omega. rewrite H. rewrite c_shift_sub. clear c_shift_sub.
-  f_equal. f_equal. f_equal. all: try omega.
+  rewrite (v_shift_comm_aux 1 j). rewrite (v_shift_comm_aux 1 (1+j)). simpl.
+  rewrite c_shift_sub. clear c_shift_sub.
+  f_equal. f_equal. all: try omega.
   rewrite <-(v_shift_shift 1 1 0). rewrite (v_shift_comm_aux 1 j).
-  rewrite (v_shift_comm_aux 1 (j+1)). f_equal. rewrite (v_shift_comm_aux 1 i).
-  rewrite (v_shift_comm_aux 1 (i+1)). f_equal. f_equal. all: omega.
+  rewrite (v_shift_comm_aux 1 (1+j)). f_equal. rewrite (v_shift_comm_aux 1 i).
+  rewrite (v_shift_comm_aux 1 (1+i)). f_equal. f_equal. all: omega.
 + clear v_shift_sub h_shift_sub.
   unfold c_sub in c_shift_sub. rewrite v_shift_comm_aux. rewrite c_shift_sub.
   f_equal. f_equal. f_equal. rewrite (v_shift_comm_aux 1 j). f_equal.
@@ -388,123 +435,11 @@ induction h; unfold h_sub; simpl. auto. f_equal.
 + apply h_shift_sub. assumption.
 + clear v_shift_sub h_shift_sub.
   unfold c_sub in c_shift_sub. rewrite <-(v_shift_shift 1).
-  rewrite (v_shift_comm_aux 1 j). rewrite (v_shift_comm_aux 1 (j+1)).
-  assert (j+1+1=j+2) by omega. rewrite H. rewrite c_shift_sub. clear c_shift_sub.
-  f_equal. f_equal. f_equal. all: try omega.
+  rewrite (v_shift_comm_aux 1 j). rewrite (v_shift_comm_aux 1 (1+j)). simpl.
+  rewrite c_shift_sub. clear c_shift_sub.
+  f_equal. f_equal. all: try omega.
   rewrite <-(v_shift_shift 1 1 0). rewrite (v_shift_comm_aux 1 j).
-  rewrite (v_shift_comm_aux 1 (j+1)). f_equal. rewrite (v_shift_comm_aux 1 i).
-  rewrite (v_shift_comm_aux 1 (i+1)). f_equal. f_equal. all: omega.
+  rewrite (v_shift_comm_aux 1 (1+j)). f_equal. rewrite (v_shift_comm_aux 1 i).
+  rewrite (v_shift_comm_aux 1 (1+i)). f_equal. f_equal. all: omega.
 }
 Qed.
-
-
-(* 
-Lemma v_shift_sub v v' i j (safe: i < j): 
-  Sub.v_shift (v_sub v v' j) 1 i = 
-  (v_sub (Sub.v_shift v 1 i) (Sub.v_shift v' 1 i) (j+1))
-with c_shift_sub c v' i j (safe: i < j): 
-  Sub.c_shift (c_sub c v' j) 1 i = 
-  (c_sub (Sub.c_shift c 1 i) (Sub.v_shift v' 1 i) (j+1))
-with h_shift_sub h v' i j (safe: i < j): 
-  Sub.h_shift (h_sub h v' j) 1 i = 
-  (h_sub (Sub.h_shift h 1 i) (Sub.v_shift v' 1 i) (j+1)).
-Proof.
-{
-induction v; unfold v_sub; simpl.
-{
-clear v_shift_sub c_shift_sub h_shift_sub.
-destruct v as (x, n). destruct (n=?j) eqn:nj.
-+ apply Nat.eqb_eq in nj. subst.
-  assert (i<=?j=true) by (apply leb_correct; omega).
-  rewrite H. simpl. assert (j+1=?j+1=true) by (apply Nat.eqb_eq; omega).
-  rewrite H0. rewrite v_negshift_shift. rewrite v_negshift_shift.
-  assert (1-1=0) by omega. rewrite H1. rewrite v_shift_0. rewrite v_shift_0.
-  reflexivity. omega. omega.
-+ destruct (i<=?n) eqn:iln; simpl.
-  - destruct (j<=?n) eqn:jln; simpl.
-    * assert (i<=?n-1=true). all: apply leb_complete in jln.
-      { apply leb_complete in iln. 
-        apply leb_correct. omega. }
-      rewrite H. assert (n+1=?j+1=false).
-      { apply Nat.eqb_neq. apply Nat.eqb_neq in nj. omega. }
-      rewrite H0. simpl. assert (j+1<=?n+1=true).
-      { apply leb_correct. omega. }
-      rewrite H1. f_equal. f_equal. assert (n>0) by omega. omega.
-    * rewrite iln. assert (n+1=?j+1=false).
-      { apply Nat.eqb_neq. apply Nat.eqb_neq in nj. omega. }
-      rewrite H. simpl. assert (j+1<=?n+1=false).
-      { apply leb_correct_conv. apply leb_complete_conv in jln. omega. }
-      rewrite H0. reflexivity.
-  - apply leb_complete_conv in iln. apply Nat.eqb_neq in nj.
-    assert (j<=?n=false) by (apply leb_correct_conv; omega).
-    rewrite H. assert (n=?j+1=false) by (apply Nat.eqb_neq; omega).
-    rewrite H0. simpl. assert (i<=?n=false) by (apply leb_correct_conv;omega).
-    rewrite H1. assert (j+1<=?n=false) by (apply leb_correct_conv; omega).
-    rewrite H2. reflexivity.
-}     
-all: f_equal; auto.
-+ clear v_shift_sub h_shift_sub.
-  unfold c_sub in c_shift_sub. rewrite v_shift_comm_aux. rewrite c_shift_sub.
-  f_equal. f_equal. f_equal. rewrite (v_shift_comm_aux 1 (j+1)). f_equal.
-  rewrite (v_shift_comm_aux 1 i). f_equal. all: omega.
-+ clear v_shift_sub h_shift_sub.
-  unfold c_sub in c_shift_sub. rewrite v_shift_comm_aux. rewrite c_shift_sub.
-  f_equal. f_equal. f_equal. rewrite (v_shift_comm_aux 1 (j+1)). f_equal.
-  rewrite (v_shift_comm_aux 1 i). f_equal. all: omega.
-+ apply h_shift_sub. auto.
-}{
-induction c; unfold c_sub; simpl; f_equal;
-try apply v_shift_sub; try assumption.
-+ clear v_shift_sub h_shift_sub.
-  unfold c_sub in c_shift_sub. rewrite <-(v_shift_shift 1).
-  rewrite (v_shift_comm_aux 1 j). rewrite (v_shift_comm_aux 1 (j+1)).
-  assert (j+1+1=j+2) by omega. rewrite H. rewrite c_shift_sub. clear c_shift_sub.
-  f_equal. f_equal. f_equal. all: try omega.
-  rewrite <-(v_shift_shift 1 1 0). rewrite (v_shift_comm_aux 1 (j+1)).
-  rewrite (v_shift_comm_aux 1 (j+1+1)). f_equal. rewrite (v_shift_comm_aux 1 i).
-  rewrite (v_shift_comm_aux 1 (i+1)). f_equal. all: omega.
-+ clear v_shift_sub h_shift_sub.
-  unfold c_sub in c_shift_sub. rewrite v_shift_comm_aux. rewrite c_shift_sub.
-  f_equal. f_equal. f_equal. rewrite (v_shift_comm_aux 1 (j+1)). f_equal.
-  rewrite (v_shift_comm_aux 1 i). f_equal. all: omega.
-+ clear v_shift_sub h_shift_sub.
-  unfold c_sub in c_shift_sub. rewrite v_shift_comm_aux. rewrite c_shift_sub.
-  f_equal. f_equal. f_equal. rewrite (v_shift_comm_aux 1 (j+1)). f_equal.
-  rewrite (v_shift_comm_aux 1 i). f_equal. all: omega.
-+ clear v_shift_sub h_shift_sub.
-  unfold c_sub in c_shift_sub. rewrite v_shift_comm_aux. rewrite c_shift_sub.
-  f_equal. f_equal. f_equal. rewrite (v_shift_comm_aux 1 (j+1)). f_equal.
-  rewrite (v_shift_comm_aux 1 i). f_equal. all: omega.
-+ clear v_shift_sub h_shift_sub.
-  unfold c_sub in c_shift_sub. rewrite <-(v_shift_shift 1).
-  rewrite (v_shift_comm_aux 1 j). rewrite (v_shift_comm_aux 1 (j+1)).
-  assert (j+1+1=j+2) by omega. rewrite H. rewrite c_shift_sub. clear c_shift_sub.
-  f_equal. f_equal. f_equal. all: try omega.
-  rewrite <-(v_shift_shift 1 1 0). rewrite (v_shift_comm_aux 1 (j+1)).
-  rewrite (v_shift_comm_aux 1 (j+1+1)). f_equal. rewrite (v_shift_comm_aux 1 i).
-  rewrite (v_shift_comm_aux 1 (i+1)). f_equal. all: omega.
-+ clear v_shift_sub h_shift_sub.
-  unfold c_sub in c_shift_sub. rewrite v_shift_comm_aux. rewrite c_shift_sub.
-  f_equal. f_equal. f_equal. rewrite (v_shift_comm_aux 1 (j+1)). f_equal.
-  rewrite (v_shift_comm_aux 1 i). f_equal. all: omega.
-+ clear v_shift_sub h_shift_sub.
-  unfold c_sub in c_shift_sub. rewrite v_shift_comm_aux. rewrite c_shift_sub.
-  f_equal. f_equal. f_equal. rewrite (v_shift_comm_aux 1 (j+1)). f_equal.
-  rewrite (v_shift_comm_aux 1 i). f_equal. all: omega.
-}{
-induction h; unfold h_sub; simpl. auto. f_equal.
-+ apply h_shift_sub. assumption.
-+ clear v_shift_sub h_shift_sub.
-  unfold c_sub in c_shift_sub. rewrite <-(v_shift_shift 1).
-  rewrite (v_shift_comm_aux 1 j). rewrite (v_shift_comm_aux 1 (j+1)).
-  assert (j+1+1=j+2) by omega. rewrite H. rewrite c_shift_sub. clear c_shift_sub.
-  f_equal. f_equal. f_equal. all: try omega.
-  rewrite <-(v_shift_shift 1 1 0). rewrite (v_shift_comm_aux 1 (j+1)).
-  rewrite (v_shift_comm_aux 1 (j+1+1)). f_equal. rewrite (v_shift_comm_aux 1 i).
-  rewrite (v_shift_comm_aux 1 (i+1)). f_equal. all: omega.
-}
-Qed.
-
-
-
- *)
